refactor cancellation  to reduce compile time

cancellation/HModInline.v
@@ -8,6 +8,8 @@ Require Import PCM IPM.
 Require Import Any.
 Require Export STB.
 Require Import Events HMod.
+Require Import SMod2HMod HMod2Mod MainAdequacy ISim.
+
 
 Set Implicit Arguments.
 
@@ -239,3 +241,161 @@ Module HIRed.
 
   End RED.
 End HIRed.
+
+
+Section CANCEL.
+  Context `{Σ: GRA.t}.
+  Notation iProp := (iProp Σ).
+
+  Lemma wrap_elimI_well_scoped
+      ms fn sb
+      (FIND: alist_find fn ms.(HModSem.fnsems) = Some sb)
+    :
+    HModSem.sandbox_body (wrap_elimI ms sb)
+    = 
+    inline_hp_fun (prog ms) (HModSem.sandbox_body sb).
+  Proof.
+    extensionality args. 
+    unfold wrap_elimI, inline_hp_fbody. s.
+    unfold HModSem.sandbox_body, inline_hp_fun. destruct sb. s.
+    assert(SCP := ms.(HModSem.well_scoped_fns)).
+    specialize (SCP fn). rewrite/fnsems_scopes FIND in SCP.
+    
+    (* remember (HModSem.scopes ms) as scopeS. i. *)
+    rename l into scopeT. 
+    apply bisim_is_eq. move scopeT at bottom.
+    eapply (@gpaco2_init _ _ _ _ (eqitC eq false false)); eauto with paco.
+    generalize (i args) as itr. clear FIND fn i args.
+    revert_until ms. gcofix CIH. i.
+    ides itr.
+    - rewrite !HModSB.transl_ret HIRed.ret HModSB.transl_ret. gstep. econs. refl.
+    - rewrite !HModSB.transl_tau HIRed.tau !HModSB.transl_tau. 
+      gstep. econs. gstep. econs. gbase. eauto.
+    - rewrite -bind_trigger !HModSB.transl_bind.
+      destruct e.
+      {
+        assert ((@ITree.trigger (@hmodE Σ) X (inl1 a)) = trigger a) by grind. 
+        rewrite H !HModSB.transl_ag HIRed.bind_ag HModSB.transl_bind HModSB.transl_ag !bind_trigger.
+        gstep. econs. i. r.
+        rewrite HModSB.transl_tau. gstep. econs. gbase. eauto.
+      }
+      destruct p.
+      {
+        assert ((@ITree.trigger (@hmodE Σ) X (inr1 (inl1 s))) = trigger s) by grind.
+        rewrite H !HModSB.transl_sch HIRed.bind_sch HModSB.transl_bind HModSB.transl_sch !bind_trigger.
+        gstep. econs. i. r.
+        rewrite HModSB.transl_tau. gstep. econs. gbase. eauto.
+      }
+      destruct s.
+      {
+        assert ((@ITree.trigger (@hmodE Σ) X (inr1 (inr1 (inl1 c)))) = trigger c) by grind.
+        destruct c. rewrite H.
+        rewrite !HModSB.transl_call HIRed.call HModSB.transl_tau. s.
+        gstep. econs.
+        destruct (alist_find fn (HModSem.fnsems ms)) eqn: FIND.
+        { 
+          ired. assert (X:=@sandbox_well_scoped). 
+          unfold HModSem.sandbox_body. destruct p. s.
+          gbase.
+          match goal with
+          [|- _ _ (_ _ ?itr)] => assert (EX: exists itr', itr = HModSem.sandbox (HModSem.scopes ms) itr')
+          end.
+          {
+            eexists. instantiate (1:= _ >>= _). 
+            rewrite HModSB.transl_bind. f_equal.
+            { 
+              erewrite <-(@sandbox_well_scoped _ _ l); eauto. 
+              assert(SCP0 := ms.(HModSem.well_scoped_fns)).
+              specialize (SCP0 fn). rewrite/fnsems_scopes FIND in SCP0.
+              eauto.
+            }
+            extensionality x.
+            instantiate (1:= fun x => tau;;(_ x)). s.
+            rewrite HModSB.transl_tau. do 2 f_equal.
+            ired.
+            erewrite <-(@sandbox_well_scoped _ _ scopeT); eauto. 
+            instantiate (1:= fun x => HModSem.sandbox scopeT (k x)). 
+            s. refl.
+          }
+          des. rewrite EX. eapply CIH. refl.
+        }
+        ired. unfold triggerNB. ired. 
+        rewrite !HIRed.bind_core !HModSB.transl_bind HModSB.transl_core !bind_trigger.
+        gstep. econs. i. ss.
+      }
+      destruct s.
+      {
+        assert ((@ITree.trigger (@hmodE Σ) X (inr1 (inr1 (inr1 (inl1 p))))) = trigger p) by grind.
+        destruct p; rewrite H.
+        {
+          rewrite !HModSB.transl_put. des_ifs.
+          {
+            rewrite HIRed.bind_pg HModSB.transl_bind HModSB.transl_put. des_ifs; cycle 1.
+            {
+              exfalso. assert (existsb (eqb k0.1) (HModSem.scopes ms) = true).
+              {
+                eapply existsb_exists. eapply existsb_exists in Heq. des.
+                esplits; eauto.
+              }
+              rewrite H0 in Heq0. ss.
+            }
+            rewrite !bind_trigger. gstep. econs. i.
+            rewrite HModSB.transl_tau. gstep. econs. gbase; eauto. 
+          }
+          rewrite HIRed.bind_core HModSB.transl_bind HModSB.transl_core !bind_trigger. 
+          gstep. econs. i. r. 
+          rewrite HModSB.transl_tau. gstep. econs. gbase; eauto.
+        }
+        rewrite !HModSB.transl_get. des_ifs.
+        {
+          rewrite HIRed.bind_pg HModSB.transl_bind HModSB.transl_get. des_ifs; cycle 1.
+          {
+            exfalso. assert (existsb (eqb k0.1) (HModSem.scopes ms) = true).
+            {
+              eapply existsb_exists. eapply existsb_exists in Heq. des.
+              esplits; eauto.
+            }
+            rewrite H0 in Heq0. ss.
+          }
+          rewrite !bind_trigger. gstep. econs. i.
+          rewrite HModSB.transl_tau. gstep. econs. gbase; eauto. 
+        }
+        rewrite HIRed.bind_core HModSB.transl_bind HModSB.transl_core !bind_trigger. 
+        gstep. econs. i. r. 
+        rewrite HModSB.transl_tau. gstep. econs. gbase; eauto.
+      }
+      assert ((@ITree.trigger (@hmodE Σ) X (inr1 (inr1 (inr1 (inr1 c))))) = trigger c) by grind.
+      rewrite H HModSB.transl_core HIRed.bind_core HModSB.transl_bind HModSB.transl_core !bind_trigger.
+      gstep. econs. i. r.
+      rewrite HModSB.transl_tau. gstep. econs. gbase; eauto.
+    Unshelve.
+      eapply eqit__mono; eauto.
+  Qed.
+
+
+  Definition bindRR {R} RR P : nat -> alist key Any.t * R-> alist key Any.t * R -> iProp :=
+    fun nths '(st0, ret0) '(st1, ret1) => (P ∗ RR nths (st0, ret0) (st1, ret1))%I.
+
+  Definition IstRR {R} Ist : nat -> alist key Any.t * R-> alist key Any.t * R -> iProp :=
+    fun nths '(st0, ret0) '(st1, ret1) => (⌜ret0 = ret1⌝ ∗ Ist nths st0 st1)%I.
+
+  Lemma isim_RR_frame
+      fls flt my_tid is_closed r g nths
+      {R} Ist (P: iProp)
+      ps pt sti_src sti_tgt
+    :
+      (P ∗ @isim _ fls flt Ist my_tid is_closed r g R 
+            (fun nths '(sts, vs) '(stt, vt) => ⌜vs = vt⌝ ∗ Ist nths sts stt)%I
+            ps pt nths sti_src sti_tgt)  
+      ⊢ isim fls flt Ist my_tid is_closed r g 
+         (bindRR (IstRR Ist) P) ps pt nths sti_src sti_tgt.
+  Proof.
+    iIntros "[H0 H1]". iApply isim_wand. iFrame. eauto.
+  Qed.
+
+  Definition progI fl : callE ~> itree hmodE :=
+    fun _ '(Call fn args) =>
+      lbody <- (alist_find fn fl)!;;
+      lbody args.
+
+End CANCEL.
