cancellation/CancelAux0.v
@@ -1,0 +1,625 @@
+
+Require Import Coqlib.
+Require Import Behavior.
+Require Import AList.
+Require Import SMod2HMod SMod2HModAux.
+Require Import Skeleton.
+Require Import PCM IPM.
+Require Import Any.
+Require Export STB.
+Require Import ModSim ISim HPSim.
+Require Import CtxRefine CtxRefineFacts MainAdequacy ClosedAdequacy.
+Require Import SimGlobal SimGlobalFacts.
+Require Import SMod HMod Mod Events.
+Require Import HModInline ElimRel.
+Require Import Mod2ITree StRed CancelDef.
+
+(* Trivial Cases *)
+
+Section CANCEL.
+  Context `{Σ: GRA.t}.
+  Variable ginv: Sk.t -> invspec.
+  Variable stb: Sk.t -> gname -> option fspec.
+  Variable md: SMod.t.
+  Notation iProp := (iProp Σ).
+
+  Let sk: Sk.t := SMod.sk md.
+  Let ms (sk0: Sk.t) (SKINCL: incl sk sk0) (SKWF: Sk.wf sk0) := 
+    SMod.modsem md sk0.
+  Let sbtb (sk0: Sk.t) (SKINCL: incl sk sk0) (SKWF: Sk.wf sk0): alist gname (list string * fspecbody) := 
+    (ms sk0 SKINCL SKWF).(SModSem.fnsems).
+  Let _stb (sk0: Sk.t) (SKINCL: incl sk sk0) (SKWF: Sk.wf sk0): alist gname (list string * fspec) := 
+    List.map (map_snd (fun '(fn, fs) => (fn, fs.(fsb_fspec)))) (sbtb sk0 SKINCL SKWF).
+
+  Hypothesis STBCOMPLETE:
+    forall 
+      sk0 (SKINCL: incl sk sk0) (SKWF: Sk.wf sk0)
+      fn scfsp (FIND: alist_find fn (_stb sk0 SKINCL SKWF) = Some scfsp), stb sk0 fn = Some scfsp.2.
+  Hypothesis STBSOUND:
+    forall 
+      sk0 (SKINCL: incl sk sk0) (SKWF: Sk.wf sk0)
+      fn (FIND: alist_find fn (_stb sk0 SKINCL SKWF) = None),
+      (<<NONE: stb sk0 fn = None>>).
+
+  Let md_src: HMod.t := SModAux.to_hmod md.
+  Let md_tgt: HMod.t := SMod.to_hmod ginv stb md.
+
+  Import CancelTAC.
+
+  Lemma cancel_main_ret
+    sk0 (SKINCL: incl sk sk0) (SKWF: Sk.wf sk0)
+    r X (meta: X) (rs0 rt0 rs rt: Σ) v  Q cid st ps pt
+    (srcs tgts: list (itree modE Any.t))
+    (WFT: ✓ rt)
+    (LENS: cid < base.length srcs)
+    (LENT: cid < base.length tgts)
+    (RET: ∀ vret ret : Any.t, cid = 0 → Q cid meta vret ret ⊢ ⌜vret = ret⌝)
+  :
+  gpaco7 _simg (cpn7 _simg) bot7 r Any.t Any.t eq ps pt
+  (x <-
+   interp_stateE Any.t
+     (x_ <- (if Nat.eq_dec cid 0 then Ret (inr v) else triggerUB);;
+      match x_ with
+      | inl l => tau;; ITree.iter (handle_schE_callE (ModSem.prog (HModSem.to_mod (HModSemAux.inline (SModSemAux.to_hmod (SMod.modsem md sk0))) rs0))) l
+      | inr r0 => Ret r0
+      end) (Any.pair st rs ↑);; Ret x.2)
+  (x <-
+   interp_stateE Any.t
+     (x_ <- trigger (Choose Any.t)%sum;;
+      x_0 <-
+      Ret
+        (inl
+           (cid,
+            <[cid:=lr <-
+                   ITree.subst
+                     (λ x : Any.t,
+                        Ret
+                          (inl
+                             (ITree.subst
+                                (λ lr : itree hmodE Any.t + Any.t,
+                                   match lr with
+                                   | inl l => tau;; ITree.iter (handle_callE (prog (SModSem.to_hmod (ginv sk0) (stb sk0) (SMod.modsem md sk0)))) l
+                                   | inr r0 => Ret r0
+                                   end) (ITree.subst (λ v0 : Any.t, Ret (inl (ITree.subst (λ ret : Any.t, trigger (Guarantee (Q cid meta v ret));;; Ret ret) (Ret v0)))) (Ret x)))))
+                     (Ret x_);; match lr with
+                                | inl l => tau;; interp_hp l
+                                | inr r0 => Ret r0
+                                end]> tgts));;
+      match x_0 with
+      | inl l => tau;; ITree.iter (handle_schE_callE (ModSem.prog (HModSem.to_mod (HModSemAux.inline (SModSem.to_hmod (ginv sk0) (stb sk0) (SMod.modsem md sk0))) rt0))) l
+      | inr r0 => Ret r0
+      end) (Any.pair st rt ↑);; Ret x.2)
+  .
+  Proof. 
+    hide_r. des_ifs; cycle 1.
+    { unfold triggerUB. ired. _coreA. }
+    ired. reveal ITREE.
+    _coreA. iterT 2. 
+    iterL. _supd. iterL. _coreA. ls.
+    iterL. _coreA. ls. iterL. _supd. iterL. _supd.
+    iterT 2. iterL. rewrite !StRed.ret. ired. st.
+    hexploit Own_bupd_split; eauto. i. des.
+    specialize (RET v x ltac:(refl)).
+    eapply Own_pure_soundness with (x := a1).
+    {
+      eapply Own_bupd_valid in WFT; eauto.
+      eapply cmra_valid_op_l; eauto.
+    }
+    etrans; eauto.
+  Qed.
+
+  Lemma cancel_main_tau
+    sk0 (SKINCL: incl sk sk0) (SKWF: Sk.wf sk0)
+    X (meta: X) (rs0 rt0 rs rt: Σ) Q cid st ps pt l
+    srcs tgts itrS itrT
+    (LENS: cid < base.length srcs)
+    (LENT: cid < base.length tgts)
+    (LEN: base.length srcs = base.length tgts)
+    (WF: ✓ rs)
+    (UPD: Own rs ==∗ Own rt)
+    (RET: ∀ vret ret : Any.t, cid = 0 → Q cid meta vret ret ⊢ ⌜vret = ret⌝)
+    (ITR: upaco3 (@elim_rel_def _ ginv stb sk0 _) bot3 l itrS itrT)
+    (RELS: ∀ (k : nat) (x y : itree modE Any.t), cid ≠ k → srcs !! k = Some x → tgts !! k = Some y → thread_rel ginv stb md sk0 cid k x y)
+    (r: ∀ x x0 : Type, (x → x0 → Prop) → smj → smj → itree coreE x → itree coreE x0 → Prop)
+    (CIH: ∀ (rs rt : Σ) (srcs tgts : list (itree modE Any.t)) (cid : nat) (st : Any.t) (ps pt : smj),
+          ✓ rs → cid < base.length srcs → (Own rs ==∗ Own rt) 
+          → ∀ src tgt : itree modE Any.t,
+            srcs !! cid = Some src → tgts !! cid = Some tgt
+            → ∀ (X : Type) (meta : X) (Q : nat → X → Any.t → Any.t → iProp) (l : list (nat * {X0 : Type & X0})) (itrS itrT : itree hmodE Any.t),
+              (∀ vret ret : Any.t, cid = 0 → Q cid meta vret ret ⊢ ⌜vret = ret⌝) 
+              → paco3 (@elim_rel_def _ ginv stb sk0 _)  bot3 l itrS itrT
+              → src = (if Nat.eq_dec cid cid then Ret () else tau;; Ret ());;; interp_hp itrS
+              → tgt = interp_hp ((if Nat.eq_dec cid cid then Ret () else yield_post ginv sk0);;; vret <- itrT;; inline_hp (prog (SModSem.to_hmod (ginv sk0) (stb sk0) (SMod.modsem md sk0))) (ret <- trigger (Choose Any.t);; trigger (Guarantee (Q cid meta vret ret));;; Ret ret))
+              → base.length srcs = base.length tgts
+              → cid < base.length tgts
+              → (∀ (k : nat) (x y : itree modE Any.t), cid ≠ k → srcs !! k = Some x → tgts !! k = Some y → thread_rel ginv stb md sk0 cid k x y)
+              → r Any.t Any.t eq ps pt
+                  (x <- interp_stateE Any.t (ITree.iter (handle_schE_callE (ModSem.prog (HModSem.to_mod (HModSemAux.inline (SModSemAux.to_hmod (SMod.modsem md sk0))) rs0))) (cid, srcs)) (Any.pair st rs ↑);; Ret x.2)
+                  (x <- interp_stateE Any.t (ITree.iter (handle_schE_callE (ModSem.prog (HModSem.to_mod (HModSemAux.inline (SModSem.to_hmod (ginv sk0) (stb sk0) (SMod.modsem md sk0))) rt0))) (cid, tgts)) (Any.pair st rt ↑);; Ret x.2))
+  :
+  gpaco7 _simg (cpn7 _simg) bot7 r Any.t Any.t eq ps pt
+  (x <- interp_stateE Any.t (tau;; tau;; ITree.iter (handle_schE_callE (ModSem.prog (HModSem.to_mod (HModSemAux.inline (SModSemAux.to_hmod (SMod.modsem md sk0))) rs0)))
+    (cid, <[cid:=interp_hp itrS]> srcs)) (Any.pair st rs ↑);; Ret x.2)
+  (x <- interp_stateE Any.t (tau;; tau;; ITree.iter (handle_schE_callE (ModSem.prog (HModSem.to_mod (HModSemAux.inline (SModSem.to_hmod (ginv sk0) (stb sk0) (SMod.modsem md sk0))) rt0)))
+    (cid, <[cid:=interp_hp (vret <- itrT;; inline_hp (prog (SModSem.to_hmod (ginv sk0) (stb sk0) (SMod.modsem md sk0))) (ret <- trigger (Choose Any.t);; trigger (Guarantee (Q cid meta vret ret));;; Ret ret))]> tgts)) (Any.pair st rt ↑);; Ret x.2).
+  Proof.
+    tau 4. prb. gbase. pclearbot. 
+    eapply CIH; eauto; try (rewrite !length_insert; nia); try (rewrite list_lookup_insert; grind).
+    i. rewrite !list_lookup_insert_ne in H0, H1; eauto.
+  Qed.
+  
+  Lemma cancel_main_core
+    sk0 (SKINCL: incl sk sk0) (SKWF: Sk.wf sk0)
+    X (meta: X) (rs0 rt0 rs rt: Σ) Q cid st ps pt l R (e:coreE R)
+    srcs tgts ktrS ktrT
+    (LENS: cid < base.length srcs)
+    (LENT: cid < base.length tgts)
+    (LEN: base.length srcs = base.length tgts)
+    (WF: ✓ rs)
+    (UPD: Own rs ==∗ Own rt)
+    (RET: ∀ vret ret : Any.t, cid = 0 → Q cid meta vret ret ⊢ ⌜vret = ret⌝)
+    (KTR: ∀ v : R, upaco3 (@elim_rel_def _ ginv stb sk0 _) bot3 l (ktrS v) (ktrT v))
+    (RELS: ∀ (k : nat) (x y : itree modE Any.t), cid ≠ k → srcs !! k = Some x → tgts !! k = Some y → thread_rel ginv stb md sk0 cid k x y)
+    (r: ∀ x x0 : Type, (x → x0 → Prop) → smj → smj → itree coreE x → itree coreE x0 → Prop)
+    (CIH: ∀ (rs rt : Σ) (srcs tgts : list (itree modE Any.t)) (cid : nat) (st : Any.t) (ps pt : smj),
+          ✓ rs → cid < base.length srcs → (Own rs ==∗ Own rt) 
+          → ∀ src tgt : itree modE Any.t,
+            srcs !! cid = Some src → tgts !! cid = Some tgt
+            → ∀ (X : Type) (meta : X) (Q : nat → X → Any.t → Any.t → iProp) (l : list (nat * {X0 : Type & X0})) (itrS itrT : itree hmodE Any.t),
+              (∀ vret ret : Any.t, cid = 0 → Q cid meta vret ret ⊢ ⌜vret = ret⌝) 
+              → paco3 (@elim_rel_def _ ginv stb sk0 _)  bot3 l itrS itrT
+              → src = (if Nat.eq_dec cid cid then Ret () else tau;; Ret ());;; interp_hp itrS
+              → tgt = interp_hp ((if Nat.eq_dec cid cid then Ret () else yield_post ginv sk0);;; vret <- itrT;; inline_hp (prog (SModSem.to_hmod (ginv sk0) (stb sk0) (SMod.modsem md sk0))) (ret <- trigger (Choose Any.t);; trigger (Guarantee (Q cid meta vret ret));;; Ret ret))
+              → base.length srcs = base.length tgts
+              → cid < base.length tgts
+              → (∀ (k : nat) (x y : itree modE Any.t), cid ≠ k → srcs !! k = Some x → tgts !! k = Some y → thread_rel ginv stb md sk0 cid k x y)
+              → r Any.t Any.t eq ps pt
+                  (x <- interp_stateE Any.t (ITree.iter (handle_schE_callE (ModSem.prog (HModSem.to_mod (HModSemAux.inline (SModSemAux.to_hmod (SMod.modsem md sk0))) rs0))) (cid, srcs)) (Any.pair st rs ↑);; Ret x.2)
+                  (x <- interp_stateE Any.t (ITree.iter (handle_schE_callE (ModSem.prog (HModSem.to_mod (HModSemAux.inline (SModSem.to_hmod (ginv sk0) (stb sk0) (SMod.modsem md sk0))) rt0))) (cid, tgts)) (Any.pair st rt ↑);; Ret x.2))
+  :
+  gpaco7 _simg (cpn7 _simg) bot7 r Any.t Any.t eq ps pt
+  (x <- interp_stateE Any.t 
+    (x_ <- trigger e;;
+      x_0 <- Ret (inl (cid, <[cid:=lr <- ITree.subst (λ x : R, Ret (inl (ITree.subst ktrS (Ret x)))) (Ret x_);; 
+                              match lr with
+                              | inl l0 => tau;; interp_hp l0
+                              | inr r0 => Ret r0
+                              end]> srcs));;
+      match x_0 with
+      | inl l0 => tau;; ITree.iter (handle_schE_callE (ModSem.prog (HModSem.to_mod (HModSemAux.inline (SModSemAux.to_hmod (SMod.modsem md sk0))) rs0))) l0
+      | inr r0 => Ret r0
+      end) (Any.pair st rs ↑);; Ret x.2)
+  (x <- interp_stateE Any.t
+    (x_ <- trigger e;;
+      x_0 <- Ret (inl (cid, <[cid:=lr <- ITree.subst (λ x : R, Ret (inl (vret <- ITree.subst (λ a : R, ktrT a) (Ret x);;
+                                                                                  inline_hp (prog (SModSem.to_hmod (ginv sk0) (stb sk0) (SMod.modsem md sk0)))
+                                                                                  (ret <- trigger (Choose Any.t);; trigger (Guarantee (Q cid meta vret ret));;; Ret ret)))) (Ret x_);;
+                              match lr with
+                              | inl l0 => tau;; interp_hp l0
+                              | inr r0 => Ret r0
+                              end]> tgts));;
+      match x_0 with
+      | inl l0 => tau;; ITree.iter (handle_schE_callE (ModSem.prog (HModSem.to_mod (HModSemAux.inline (SModSem.to_hmod (ginv sk0) (stb sk0) (SMod.modsem md sk0))) rt0))) l0
+      | inr r0 => Ret r0
+      end) (Any.pair st rt ↑);; Ret x.2).
+  Proof.
+  depdes e.
+  - hide_l. _coreA. iterT 1.
+    reveal ITREE. hide_r. _coreE x. iterT 1.
+    reveal ITREE. prb. gbase. pclearbot.
+    eapply CIH; eauto; try (rewrite !length_insert; nia); try (rewrite list_lookup_insert; grind).
+    i. rewrite !list_lookup_insert_ne in H0, H1; eauto.
+  - hide_r. _coreA. iterT 1.
+    reveal ITREE. hide_l. _coreE x. iterT 1. 
+    reveal ITREE. prb. gbase. pclearbot.
+    eapply CIH; eauto; try (rewrite !length_insert; nia); try (rewrite list_lookup_insert; grind).
+    i. rewrite !list_lookup_insert_ne in H0, H1; eauto.
+  - hide_l. _core. reveal ITREE. hide_r. _core. reveal ITREE. st. instantiate (1:= smj_top). i. subst. 
+    hide_l. st. ired. tau 1. iterT 1.
+    reveal ITREE. hide_r. st. ired. tau 1. iterT 1.
+    reveal ITREE. prb. gbase. pclearbot.
+    eapply CIH; eauto; try (rewrite !length_insert; nia); try (rewrite list_lookup_insert; grind).
+    i. rewrite !list_lookup_insert_ne in H0, H1; eauto.
+  Qed.
+
+  Lemma cancel_main_pg
+    sk0 (SKINCL: incl sk sk0) (SKWF: Sk.wf sk0)
+    X (meta: X) (rs0 rt0 rs rt: Σ) Q cid st ps pt l R (e:pgE R)
+    srcs tgts ktrS ktrT
+    (LENS: cid < base.length srcs)
+    (LENT: cid < base.length tgts)
+    (LEN: base.length srcs = base.length tgts)
+    (WF: ✓ rs)
+    (UPD: Own rs ==∗ Own rt)
+    (RET: ∀ vret ret : Any.t, cid = 0 → Q cid meta vret ret ⊢ ⌜vret = ret⌝)
+    (KTR: ∀ v : R, upaco3 (@elim_rel_def _ ginv stb sk0 _) bot3 l (ktrS v) (ktrT v))
+    (RELS: ∀ (k : nat) (x y : itree modE Any.t), cid ≠ k → srcs !! k = Some x → tgts !! k = Some y → thread_rel ginv stb md sk0 cid k x y)
+    (r: ∀ x x0 : Type, (x → x0 → Prop) → smj → smj → itree coreE x → itree coreE x0 → Prop)
+    (CIH: ∀ (rs rt : Σ) (srcs tgts : list (itree modE Any.t)) (cid : nat) (st : Any.t) (ps pt : smj),
+          ✓ rs → cid < base.length srcs → (Own rs ==∗ Own rt) 
+          → ∀ src tgt : itree modE Any.t,
+            srcs !! cid = Some src → tgts !! cid = Some tgt
+            → ∀ (X : Type) (meta : X) (Q : nat → X → Any.t → Any.t → iProp) (l : list (nat * {X0 : Type & X0})) (itrS itrT : itree hmodE Any.t),
+              (∀ vret ret : Any.t, cid = 0 → Q cid meta vret ret ⊢ ⌜vret = ret⌝) 
+              → paco3 (@elim_rel_def _ ginv stb sk0 _)  bot3 l itrS itrT
+              → src = (if Nat.eq_dec cid cid then Ret () else tau;; Ret ());;; interp_hp itrS
+              → tgt = interp_hp ((if Nat.eq_dec cid cid then Ret () else yield_post ginv sk0);;; vret <- itrT;; inline_hp (prog (SModSem.to_hmod (ginv sk0) (stb sk0) (SMod.modsem md sk0))) (ret <- trigger (Choose Any.t);; trigger (Guarantee (Q cid meta vret ret));;; Ret ret))
+              → base.length srcs = base.length tgts
+              → cid < base.length tgts
+              → (∀ (k : nat) (x y : itree modE Any.t), cid ≠ k → srcs !! k = Some x → tgts !! k = Some y → thread_rel ginv stb md sk0 cid k x y)
+              → r Any.t Any.t eq ps pt
+                  (x <- interp_stateE Any.t (ITree.iter (handle_schE_callE (ModSem.prog (HModSem.to_mod (HModSemAux.inline (SModSemAux.to_hmod (SMod.modsem md sk0))) rs0))) (cid, srcs)) (Any.pair st rs ↑);; Ret x.2)
+                  (x <- interp_stateE Any.t (ITree.iter (handle_schE_callE (ModSem.prog (HModSem.to_mod (HModSemAux.inline (SModSem.to_hmod (ginv sk0) (stb sk0) (SMod.modsem md sk0))) rt0))) (cid, tgts)) (Any.pair st rt ↑);; Ret x.2))
+  :
+  gpaco7 _simg (cpn7 _simg) bot7 r Any.t Any.t eq ps pt
+  (x <- interp_stateE Any.t
+    (x_ <- match _observe 
+                          (match observe (ITree.map (λ x : R, inl (ITree.subst ktrS (Ret x))) (handle_pgE e)) with
+                          | RetF r0 => 
+                            match r0 with
+                            | inl l0 => tau;; interp_hp l0
+                            | inr r1 => Ret r1
+                            end
+                          | TauF t => tau;; lr <- t;; 
+                            match lr with
+                            | inl l0 => tau;; interp_hp l0
+                            | inr r0 => Ret r0
+                            end
+                          | @VisF _ _ _ X0 e1 h => Vis e1 (λ x : X0, lr <- h x;; 
+                            match lr with
+                            | inl l0 => tau;; interp_hp l0
+                            | inr r0 => Ret r0
+                            end)
+                          end) 
+           with
+          | RetF rv => if Nat.eq_dec cid 0 then Ret (inr rv) else triggerUB
+          | TauF itr' => tau;; Ret (inl (cid, <[cid:=itr']> srcs))
+          | @VisF _ _ _ X0 e1 k =>
+            match e1 with
+            | (e2|)%sum =>
+                match e2 in (schE T) return ((T → itree modE Any.t) → itree (stateE +' coreE) (nat * list (itree modE Any.t) + Any.t)) with
+                | Spawn fn arg =>
+                    λ k0 : nat → itree modE Any.t,
+                      Ret
+                        (inl
+                           (cid,
+                            <[cid:=k0 (base.length srcs)]> srcs ++
+                            [sem <-
+                             (alist_find fn
+                                (List.map (map_snd (interp_hp_fun ∘ HModSem.sandbox_body))
+                                   (List.map (map_snd (wrap_elimI (SModSemAux.to_hmod (SMod.modsem md sk0))))
+                                      (List.map (map_snd (λ ksb : list string * fspecbody, (ksb.1, interp_sb_hp_aux ksb.2))) (SModSem.fnsems (SMod.modsem md sk0)))))) !;; 
+                             sem arg]))
+                | Yield tid' => λ k0 : () → itree modE Any.t, Ret (inl (tid', <[cid:=k0 ()]> srcs))
+                | Tid => λ k0 : nat → itree modE Any.t, Ret (inl (cid, <[cid:=k0 cid]> srcs))
+                end k
+            | (|s)%sum =>
+                match s with
+                | (e2|)%sum => Ret (inl (cid, <[cid:=x <- ModSem.prog (HModSem.to_mod (HModSemAux.inline (SModSemAux.to_hmod (SMod.modsem md sk0))) rs0) e2;; (tau;; k x)]> srcs))
+                | (|e2)%sum => v <- trigger e2;; Ret (inl (cid, <[cid:=k v]> srcs))
+                end
+            end
+          end;;
+          match x_ with
+          | inl l0 => tau;; ITree.iter (handle_schE_callE (ModSem.prog (HModSem.to_mod (HModSemAux.inline (SModSemAux.to_hmod (SMod.modsem md sk0))) rs0))) l0
+          | inr r0 => Ret r0
+          end) (Any.pair st rs ↑);; Ret x.2)
+  (x <-
+   interp_stateE Any.t
+     (x_ <-
+      match
+        _observe
+          match
+            observe
+              (ITree.map
+                 (λ x : R,
+                    inl
+                      (vret <- ITree.subst (λ a : R, ktrT a) (Ret x);;
+                       inline_hp (prog (SModSem.to_hmod (ginv sk0) (stb sk0) (SMod.modsem md sk0)))
+                         (ret <- trigger (Choose Any.t);; trigger (Guarantee (Q cid meta vret ret));;; Ret ret))) (handle_pgE e))
+          with
+          | RetF r0 => match r0 with
+                       | inl l0 => tau;; interp_hp l0
+                       | inr r1 => Ret r1
+                       end
+          | TauF t => tau;; lr <- t;; match lr with
+                                      | inl l0 => tau;; interp_hp l0
+                                      | inr r0 => Ret r0
+                                      end
+          | @VisF _ _ _ X0 e1 h => Vis e1 (λ x : X0, lr <- h x;; match lr with
+                                                                 | inl l0 => tau;; interp_hp l0
+                                                                 | inr r0 => Ret r0
+                                                                 end)
+          end
+      with
+      | RetF rv => if Nat.eq_dec cid 0 then Ret (inr rv) else triggerUB
+      | TauF itr' => tau;; Ret (inl (cid, <[cid:=itr']> tgts))
+      | @VisF _ _ _ X0 e1 k =>
+          match e1 with
+          | (e2|)%sum =>
+              match e2 in (schE T) return ((T → itree modE Any.t) → itree (stateE +' coreE) (nat * list (itree modE Any.t) + Any.t)) with
+              | Spawn fn arg =>
+                  λ k0 : nat → itree modE Any.t,
+                    Ret
+                      (inl
+                         (cid,
+                          <[cid:=k0 (base.length tgts)]> tgts ++
+                          [sem <-
+                           (alist_find fn
+                              (List.map (map_snd (interp_hp_fun ∘ HModSem.sandbox_body))
+                                 (List.map (map_snd (wrap_elimI (SModSem.to_hmod (ginv sk0) (stb sk0) (SMod.modsem md sk0))))
+                                    (List.map (map_snd (λ ksb : list string * fspecbody, (ksb.1, interp_sb_hp (ginv sk0) (stb sk0) ksb.2))) (SModSem.fnsems (SMod.modsem md sk0))))))
+                           !;; sem arg]))
+              | Yield tid' => λ k0 : () → itree modE Any.t, Ret (inl (tid', <[cid:=k0 ()]> tgts))
+              | Tid => λ k0 : nat → itree modE Any.t, Ret (inl (cid, <[cid:=k0 cid]> tgts))
+              end k
+          | (|s)%sum =>
+              match s with
+              | (e2|)%sum =>
+                  Ret
+                    (inl
+                       (cid, <[cid:=x <- ModSem.prog (HModSem.to_mod (HModSemAux.inline (SModSem.to_hmod (ginv sk0) (stb sk0) (SMod.modsem md sk0))) rt0) e2;; (tau;; k x)]> tgts))
+              | (|e2)%sum => v <- trigger e2;; Ret (inl (cid, <[cid:=k v]> tgts))
+              end
+          end
+      end;;
+      match x_ with
+      | inl l0 => tau;; ITree.iter (handle_schE_callE (ModSem.prog (HModSem.to_mod (HModSemAux.inline (SModSem.to_hmod (ginv sk0) (stb sk0) (SMod.modsem md sk0))) rt0))) l0
+      | inr r0 => Ret r0
+      end) (Any.pair st rt ↑);; Ret x.2).
+  Proof.
+    depdes e.
+    - hide_l. grind. _supd. iterL. _supd. iterT 1.
+      reveal ITREE. hide_r. 
+      grind. _supd. iterL. _supd. iterT 1.
+      reveal ITREE. prb. gbase. pclearbot.
+      eapply CIH; eauto; try (rewrite !length_insert; nia); try (rewrite list_lookup_insert; grind).
+      i. rewrite !list_lookup_insert_ne in H0, H1; eauto.
+    - hide_l. grind. _supd. iterT 1.
+      reveal ITREE. hide_r.
+      grind. _supd. iterT 1.
+      reveal ITREE. prb. gbase. pclearbot.
+      eapply CIH; eauto; try (rewrite !length_insert; nia); try (rewrite list_lookup_insert; grind).
+      i. rewrite !list_lookup_insert_ne in H0, H1; eauto.
+  Qed.
+
+  Lemma cancel_main_asm
+    sk0 (SKINCL: incl sk sk0) (SKWF: Sk.wf sk0)
+    X (meta: X) (rs0 rt0 rs rt: Σ) Q cid st ps pt l P
+    srcs tgts ktrS ktrT
+    (LENS: cid < base.length srcs)
+    (LENT: cid < base.length tgts)
+    (LEN: base.length srcs = base.length tgts)
+    (WF: ✓ rs)
+    (UPD: Own rs ==∗ Own rt)
+    (RET: ∀ vret ret : Any.t, cid = 0 → Q cid meta vret ret ⊢ ⌜vret = ret⌝)
+    (KTR: upaco3 (@elim_rel_def _ ginv stb sk0 _) bot3 l (ktrS ()) (ktrT ()))
+    (RELS: ∀ (k : nat) (x y : itree modE Any.t), cid ≠ k → srcs !! k = Some x → tgts !! k = Some y → thread_rel ginv stb md sk0 cid k x y)
+    (r: ∀ x x0 : Type, (x → x0 → Prop) → smj → smj → itree coreE x → itree coreE x0 → Prop)
+    (CIH: ∀ (rs rt : Σ) (srcs tgts : list (itree modE Any.t)) (cid : nat) (st : Any.t) (ps pt : smj),
+          ✓ rs → cid < base.length srcs → (Own rs ==∗ Own rt) 
+          → ∀ src tgt : itree modE Any.t,
+            srcs !! cid = Some src → tgts !! cid = Some tgt
+            → ∀ (X : Type) (meta : X) (Q : nat → X → Any.t → Any.t → iProp) (l : list (nat * {X0 : Type & X0})) (itrS itrT : itree hmodE Any.t),
+              (∀ vret ret : Any.t, cid = 0 → Q cid meta vret ret ⊢ ⌜vret = ret⌝) 
+              → paco3 (@elim_rel_def _ ginv stb sk0 _)  bot3 l itrS itrT
+              → src = (if Nat.eq_dec cid cid then Ret () else tau;; Ret ());;; interp_hp itrS
+              → tgt = interp_hp ((if Nat.eq_dec cid cid then Ret () else yield_post ginv sk0);;; vret <- itrT;; inline_hp (prog (SModSem.to_hmod (ginv sk0) (stb sk0) (SMod.modsem md sk0))) (ret <- trigger (Choose Any.t);; trigger (Guarantee (Q cid meta vret ret));;; Ret ret))
+              → base.length srcs = base.length tgts
+              → cid < base.length tgts
+              → (∀ (k : nat) (x y : itree modE Any.t), cid ≠ k → srcs !! k = Some x → tgts !! k = Some y → thread_rel ginv stb md sk0 cid k x y)
+              → r Any.t Any.t eq ps pt
+                  (x <- interp_stateE Any.t (ITree.iter (handle_schE_callE (ModSem.prog (HModSem.to_mod (HModSemAux.inline (SModSemAux.to_hmod (SMod.modsem md sk0))) rs0))) (cid, srcs)) (Any.pair st rs ↑);; Ret x.2)
+                  (x <- interp_stateE Any.t (ITree.iter (handle_schE_callE (ModSem.prog (HModSem.to_mod (HModSemAux.inline (SModSem.to_hmod (ginv sk0) (stb sk0) (SMod.modsem md sk0))) rt0))) (cid, tgts)) (Any.pair st rt ↑);; Ret x.2))
+  :
+  gpaco7 _simg (cpn7 _simg) bot7 r Any.t Any.t eq ps pt
+  (x <-
+   interp_stateE Any.t
+     (x_ <- trigger (Take Σ);;
+      x_0 <-
+      Ret
+        (inl
+           (cid,
+            <[cid:=lr <-
+                   ITree.subst (λ x : (), Ret (inl (ITree.subst ktrS (Ret x))))
+                     (ITree.subst (λ r0 : Σ, mr <- mget_res;; assume (✓ (r0 ⋅ mr));;; assume (Own r0 ⊢ P);;; mput_res (r0 ⋅ mr)) (Ret x_));;
+                   match lr with
+                   | inl l0 => tau;; interp_hp l0
+                   | inr r0 => Ret r0
+                   end]> srcs));;
+      match x_0 with
+      | inl l0 => tau;; ITree.iter (handle_schE_callE (ModSem.prog (HModSem.to_mod (HModSemAux.inline (SModSemAux.to_hmod (SMod.modsem md sk0))) rs0))) l0
+      | inr r0 => Ret r0
+      end) (Any.pair st rs ↑);; Ret x.2)
+  (x <-
+   interp_stateE Any.t
+     (x_ <- trigger (Take Σ);;
+      x_0 <-
+      Ret
+        (inl
+           (cid,
+            <[cid:=lr <-
+                   ITree.subst
+                     (λ x : (),
+                        Ret
+                          (inl
+                             (vret <- ITree.subst (λ a : (), ktrT a) (Ret x);;
+                              inline_hp (prog (SModSem.to_hmod (ginv sk0) (stb sk0) (SMod.modsem md sk0)))
+                                (ret <- trigger (Choose Any.t);; trigger (Guarantee (Q cid meta vret ret));;; Ret ret))))
+                     (ITree.subst (λ r0 : Σ, mr <- mget_res;; assume (✓ (r0 ⋅ mr));;; assume (Own r0 ⊢ P);;; mput_res (r0 ⋅ mr)) (Ret x_));;
+                   match lr with
+                   | inl l0 => tau;; interp_hp l0
+                   | inr r0 => Ret r0
+                   end]> tgts));;
+      match x_0 with
+      | inl l0 => tau;; ITree.iter (handle_schE_callE (ModSem.prog (HModSem.to_mod (HModSemAux.inline (SModSem.to_hmod (ginv sk0) (stb sk0) (SMod.modsem md sk0))) rt0))) l0
+      | inr r0 => Ret r0
+      end) (Any.pair st rt ↑);; Ret x.2).
+  Proof.
+    hide_r. _coreA. iterL. _supd. 
+    iterL. _coreA. iterL. _coreA.
+    iterL. _supd. iterL. _supd. iterT 1.
+    reveal ITREE. hide_l. _coreE x.
+    assert (UPD': Own(x ⋅ rs) ==∗ Own (x ⋅ rt)).
+    { iIntros "[H0 H1]". iSplitL "H0"; eauto.
+      iApply UPD; eauto.
+    }
+    assert (✓ (x ⋅ rt)). 
+    { 
+      hexploit Own_bupd_valid; eauto.
+      iIntros "H". iPoseProof (UPD' with "H") as ">[H0 H1]".
+      iModIntro. iFrame.
+    }
+    iterL. _supd. iterL. _coreE H. ls.
+    iterL. _coreE x1. ls. 
+    iterL. _supd. iterL. _supd.
+    iterT 1.
+    reveal ITREE. prb. gbase. pclearbot.
+    eapply CIH; eauto; try (rewrite !length_insert; nia); try (rewrite list_lookup_insert; grind).
+    i. rewrite !list_lookup_insert_ne in H1, H2; eauto.
+  Qed.
+
+
+
+
+  Lemma cancel_main_grt
+    sk0 (SKINCL: incl sk sk0) (SKWF: Sk.wf sk0)
+    X (meta: X) (rs0 rt0 rs rt: Σ) Q cid st ps pt l P
+    srcs tgts ktrS ktrT
+    (LENS: cid < base.length srcs)
+    (LENT: cid < base.length tgts)
+    (LEN: base.length srcs = base.length tgts)
+    (WF: ✓ rs)
+    (UPD: Own rs ==∗ Own rt)
+    (RET: ∀ vret ret : Any.t, cid = 0 → Q cid meta vret ret ⊢ ⌜vret = ret⌝)
+    (KTR: upaco3 (@elim_rel_def _ ginv stb sk0 _) bot3 l (ktrS ()) (ktrT ()))
+    (RELS: ∀ (k : nat) (x y : itree modE Any.t), cid ≠ k → srcs !! k = Some x → tgts !! k = Some y → thread_rel ginv stb md sk0 cid k x y)
+    (r: ∀ x x0 : Type, (x → x0 → Prop) → smj → smj → itree coreE x → itree coreE x0 → Prop)
+    (CIH: ∀ (rs rt : Σ) (srcs tgts : list (itree modE Any.t)) (cid : nat) (st : Any.t) (ps pt : smj),
+          ✓ rs → cid < base.length srcs → (Own rs ==∗ Own rt) 
+          → ∀ src tgt : itree modE Any.t,
+            srcs !! cid = Some src → tgts !! cid = Some tgt
+            → ∀ (X : Type) (meta : X) (Q : nat → X → Any.t → Any.t → iProp) (l : list (nat * {X0 : Type & X0})) (itrS itrT : itree hmodE Any.t),
+              (∀ vret ret : Any.t, cid = 0 → Q cid meta vret ret ⊢ ⌜vret = ret⌝) 
+              → paco3 (@elim_rel_def _ ginv stb sk0 _)  bot3 l itrS itrT
+              → src = (if Nat.eq_dec cid cid then Ret () else tau;; Ret ());;; interp_hp itrS
+              → tgt = interp_hp ((if Nat.eq_dec cid cid then Ret () else yield_post ginv sk0);;; vret <- itrT;; inline_hp (prog (SModSem.to_hmod (ginv sk0) (stb sk0) (SMod.modsem md sk0))) (ret <- trigger (Choose Any.t);; trigger (Guarantee (Q cid meta vret ret));;; Ret ret))
+              → base.length srcs = base.length tgts
+              → cid < base.length tgts
+              → (∀ (k : nat) (x y : itree modE Any.t), cid ≠ k → srcs !! k = Some x → tgts !! k = Some y → thread_rel ginv stb md sk0 cid k x y)
+              → r Any.t Any.t eq ps pt
+                  (x <- interp_stateE Any.t (ITree.iter (handle_schE_callE (ModSem.prog (HModSem.to_mod (HModSemAux.inline (SModSemAux.to_hmod (SMod.modsem md sk0))) rs0))) (cid, srcs)) (Any.pair st rs ↑);; Ret x.2)
+                  (x <- interp_stateE Any.t (ITree.iter (handle_schE_callE (ModSem.prog (HModSem.to_mod (HModSemAux.inline (SModSem.to_hmod (ginv sk0) (stb sk0) (SMod.modsem md sk0))) rt0))) (cid, tgts)) (Any.pair st rt ↑);; Ret x.2))
+  :
+  gpaco7 _simg (cpn7 _simg) bot7 r Any.t Any.t eq ps pt
+  (x <-
+   interp_stateE Any.t
+     (x_ <- trigger sGet;;
+      x_0 <-
+      Ret
+        (inl
+           (cid,
+            <[cid:=lr <-
+                   ITree.subst (λ x : (), Ret (inl (ITree.subst ktrS (Ret x))))
+                     (ITree.subst (λ mr : Σ, mr' <- trigger (Choose Σ);; guarantee (Own mr ==∗ P ∗ Own mr');;; mput_res mr')
+                        (ITree.subst (λ st0 : Any.t, x_0 <- (Any.split st0) ?;; (let (_, mr) := x_0 in (mr ↓) ?)) (Ret x_)));;
+                   match lr with
+                   | inl l0 => tau;; interp_hp l0
+                   | inr r0 => Ret r0
+                   end]> srcs));;
+      match x_0 with
+      | inl l0 => tau;; ITree.iter (handle_schE_callE (ModSem.prog (HModSem.to_mod (HModSemAux.inline (SModSemAux.to_hmod (SMod.modsem md sk0))) rs0))) l0
+      | inr r0 => Ret r0
+      end) (Any.pair st rs ↑);; Ret x.2)
+  (x <-
+   interp_stateE Any.t
+     (x_ <- trigger sGet;;
+      x_0 <-
+      Ret
+        (inl
+           (cid,
+            <[cid:=lr <-
+                   ITree.subst
+                     (λ x : (),
+                        Ret
+                          (inl
+                             (vret <- ITree.subst (λ a : (), ktrT a) (Ret x);;
+                              inline_hp (prog (SModSem.to_hmod (ginv sk0) (stb sk0) (SMod.modsem md sk0)))
+                                (ret <- trigger (Choose Any.t);; trigger (Guarantee (Q cid meta vret ret));;; Ret ret))))
+                     (ITree.subst (λ mr : Σ, mr' <- trigger (Choose Σ);; guarantee (Own mr ==∗ P ∗ Own mr');;; mput_res mr')
+                        (ITree.subst (λ st0 : Any.t, x_0 <- (Any.split st0) ?;; (let (_, mr) := x_0 in (mr ↓) ?)) (Ret x_)));;
+                   match lr with
+                   | inl l0 => tau;; interp_hp l0
+                   | inr r0 => Ret r0
+                   end]> tgts));;
+      match x_0 with
+      | inl l0 => tau;; ITree.iter (handle_schE_callE (ModSem.prog (HModSem.to_mod (HModSemAux.inline (SModSem.to_hmod (ginv sk0) (stb sk0) (SMod.modsem md sk0))) rt0))) l0
+      | inr r0 => Ret r0
+      end) (Any.pair st rt ↑);; Ret x.2).
+  Proof.
+      ired. hide_l. _supd.
+      iterL. _coreA. iterL. _coreA.
+      iterL. _supd. iterL. _supd. iterT 1.
+      reveal ITREE. hide_r. _supd.
+      assert (Own rs ==∗ P ∗ Own x).
+      {
+        iIntros "H". iPoseProof (UPD with "H") as ">H". 
+        iApply x0; eauto.
+      }
+      iterL. _coreE x. iterL. _coreE H.
+      iterL. _supd. iterL. _supd. iterT 1.
+      reveal ITREE. prb. gbase. pclearbot.
+      eapply CIH; eauto; try (rewrite !length_insert; nia); try (rewrite list_lookup_insert; grind).
+      { 
+        hexploit Own_bupd_split; eauto. i. des.
+        eapply Own_bupd_valid in H0; eauto.
+        eapply Own_pure_soundness with (x:=a2).
+        { eapply cmra_valid_op_r, Own_wand_valid; eauto. }
+        iIntros "H". iApply Own_valid. iStopProof. eauto.
+      }
+      i. rewrite !list_lookup_insert_ne in H1, H2; eauto.
+  Qed.
+
+  Lemma cancel_main_tid
+    sk0 (SKINCL: incl sk sk0) (SKWF: Sk.wf sk0)
+    X (meta: X) (rs0 rt0 rs rt: Σ) Q cid st ps pt l
+    srcs tgts ktrS ktrT
+    (LENS: cid < base.length srcs)
+    (LENT: cid < base.length tgts)
+    (LEN: base.length srcs = base.length tgts)
+    (WF: ✓ rs)
+    (UPD: Own rs ==∗ Own rt)
+    (RET: ∀ vret ret : Any.t, cid = 0 → Q cid meta vret ret ⊢ ⌜vret = ret⌝)
+    (KTR: ∀ (tid: nat), upaco3 (@elim_rel_def _ ginv stb sk0 _) bot3 l (ktrS tid) (ktrT tid))
+    (RELS: ∀ (k : nat) (x y : itree modE Any.t), cid ≠ k → srcs !! k = Some x → tgts !! k = Some y → thread_rel ginv stb md sk0 cid k x y)
+    (r: ∀ x x0 : Type, (x → x0 → Prop) → smj → smj → itree coreE x → itree coreE x0 → Prop)
+    (CIH: ∀ (rs rt : Σ) (srcs tgts : list (itree modE Any.t)) (cid : nat) (st : Any.t) (ps pt : smj),
+          ✓ rs → cid < base.length srcs → (Own rs ==∗ Own rt) 
+          → ∀ src tgt : itree modE Any.t,
+            srcs !! cid = Some src → tgts !! cid = Some tgt
+            → ∀ (X : Type) (meta : X) (Q : nat → X → Any.t → Any.t → iProp) (l : list (nat * {X0 : Type & X0})) (itrS itrT : itree hmodE Any.t),
+              (∀ vret ret : Any.t, cid = 0 → Q cid meta vret ret ⊢ ⌜vret = ret⌝) 
+              → paco3 (@elim_rel_def _ ginv stb sk0 _)  bot3 l itrS itrT
+              → src = (if Nat.eq_dec cid cid then Ret () else tau;; Ret ());;; interp_hp itrS
+              → tgt = interp_hp ((if Nat.eq_dec cid cid then Ret () else yield_post ginv sk0);;; vret <- itrT;; inline_hp (prog (SModSem.to_hmod (ginv sk0) (stb sk0) (SMod.modsem md sk0))) (ret <- trigger (Choose Any.t);; trigger (Guarantee (Q cid meta vret ret));;; Ret ret))
+              → base.length srcs = base.length tgts
+              → cid < base.length tgts
+              → (∀ (k : nat) (x y : itree modE Any.t), cid ≠ k → srcs !! k = Some x → tgts !! k = Some y → thread_rel ginv stb md sk0 cid k x y)
+              → r Any.t Any.t eq ps pt
+                  (x <- interp_stateE Any.t (ITree.iter (handle_schE_callE (ModSem.prog (HModSem.to_mod (HModSemAux.inline (SModSemAux.to_hmod (SMod.modsem md sk0))) rs0))) (cid, srcs)) (Any.pair st rs ↑);; Ret x.2)
+                  (x <- interp_stateE Any.t (ITree.iter (handle_schE_callE (ModSem.prog (HModSem.to_mod (HModSemAux.inline (SModSem.to_hmod (ginv sk0) (stb sk0) (SMod.modsem md sk0))) rt0))) (cid, tgts)) (Any.pair st rt ↑);; Ret x.2))
+  :
+  gpaco7 _simg (cpn7 _simg) bot7 r Any.t Any.t eq ps pt
+  (x <- interp_stateE Any.t (tau;; ITree.iter (handle_schE_callE (ModSem.prog (HModSem.to_mod (HModSemAux.inline (SModSemAux.to_hmod (SMod.modsem md sk0))) rs0)))
+    (cid, <[cid:=tau;; interp_hp (ktrS cid)]> srcs)) (Any.pair st rs ↑);; Ret x.2)
+  (x <- interp_stateE Any.t (tau;; ITree.iter (handle_schE_callE (ModSem.prog (HModSem.to_mod (HModSemAux.inline (SModSem.to_hmod (ginv sk0) (stb sk0) (SMod.modsem md sk0))) rt0)))
+    (cid, <[cid:=tau;; interp_hp (x_ <- ktrT cid;; inline_hp (prog (SModSem.to_hmod (ginv sk0) (stb sk0) (SMod.modsem md sk0))) (ret <- trigger (Choose Any.t);; trigger (Guarantee (Q cid meta x_ ret));;; Ret ret))]> tgts)) (Any.pair st rt ↑);; Ret x.2).
+  Proof.
+    hide_l. tau 1. iterT 1. 
+    reveal ITREE. hide_r. tau 1. iterT 1. 
+    reveal ITREE. prb. gbase. pclearbot.
+    eapply CIH; eauto; try (rewrite !length_insert; eauto); try (rewrite list_lookup_insert; grind).
+    i. rewrite !list_lookup_insert_ne in H0, H1; eauto.
+  Qed.
+
+End CANCEL.
