cancellation/CancelAux1.v
@@ -1,0 +1,209 @@
+Require Import Coqlib.
+Require Import Behavior.
+Require Import AList.
+Require Import SMod2HMod SMod2HModAux.
+Require Import Skeleton.
+Require Import PCM IPM.
+Require Import Any.
+Require Export STB.
+Require Import ModSim ISim HPSim.
+Require Import CtxRefine CtxRefineFacts MainAdequacy ClosedAdequacy.
+Require Import SimGlobal SimGlobalFacts.
+Require Import SMod HMod Mod Events.
+Require Import HModInline ElimRel.
+Require Import Mod2ITree StRed CancelDef.
+
+(* pre/post conditions of function calls *)
+
+Section CANCEL.
+  Context `{Σ: GRA.t}.
+  Variable ginv: Sk.t -> invspec.
+  Variable stb: Sk.t -> gname -> option fspec.
+  Variable md: SMod.t.
+  Notation iProp := (iProp Σ).
+
+  Let sk: Sk.t := SMod.sk md.
+  Let ms (sk0: Sk.t) (SKINCL: incl sk sk0) (SKWF: Sk.wf sk0) := 
+    SMod.modsem md sk0.
+  Let sbtb (sk0: Sk.t) (SKINCL: incl sk sk0) (SKWF: Sk.wf sk0): alist gname (list string * fspecbody) := 
+    (ms sk0 SKINCL SKWF).(SModSem.fnsems).
+  Let _stb (sk0: Sk.t) (SKINCL: incl sk sk0) (SKWF: Sk.wf sk0): alist gname (list string * fspec) := 
+    List.map (map_snd (fun '(fn, fs) => (fn, fs.(fsb_fspec)))) (sbtb sk0 SKINCL SKWF).
+
+  Hypothesis STBCOMPLETE:
+    forall 
+      sk0 (SKINCL: incl sk sk0) (SKWF: Sk.wf sk0)
+      fn scfsp (FIND: alist_find fn (_stb sk0 SKINCL SKWF) = Some scfsp), stb sk0 fn = Some scfsp.2.
+  Hypothesis STBSOUND:
+    forall 
+      sk0 (SKINCL: incl sk sk0) (SKWF: Sk.wf sk0)
+      fn (FIND: alist_find fn (_stb sk0 SKINCL SKWF) = None),
+      (<<NONE: stb sk0 fn = None>>).
+
+  Let md_src: HMod.t := SModAux.to_hmod md.
+  Let md_tgt: HMod.t := SMod.to_hmod ginv stb md.
+
+  Import CancelTAC.
+
+  Lemma cancel_main_head
+    sk0 (SKINCL: incl sk sk0) (SKWF: Sk.wf sk0)
+    X X0 (meta: X) (rs0 rt0 rs rt: Σ) P Q cid st ps pt l varg
+    src srcs tgts ktrS ktrT
+    (SRC: src = ktrS varg)
+    (LENS: cid < base.length srcs)
+    (LENT: cid < base.length tgts)
+    (LEN: base.length srcs = base.length tgts)
+    (WFS: ✓ rs)
+    (WFT: ✓ rt)
+    (UPD: Own rs ==∗ Own rt)
+    (RET: ∀ vret ret : Any.t, cid = 0 → Q cid meta vret ret ⊢ ⌜vret = ret⌝)
+    (KTR: ∀(tid: nat) (m: X0) (varg: Any.t), upaco3 (@elim_rel_def _ ginv stb sk0 _) bot3 ((tid, existT X0 m) :: l) (ktrS varg) (ktrT (tid, m, tid, m, varg)))
+    (RELS: ∀ (k : nat) (x y : itree modE Any.t), cid ≠ k → srcs !! k = Some x → tgts !! k = Some y → thread_rel ginv stb md sk0 cid k x y)
+    (r: ∀ x x0 : Type, (x → x0 → Prop) → smj → smj → itree coreE x → itree coreE x0 → Prop)
+    (CIH: ∀ (rs rt : Σ) (srcs tgts : list (itree modE Any.t)) (cid : nat) (st : Any.t) (ps pt : smj),
+          ✓ rs → cid < base.length srcs → (Own rs ==∗ Own rt) 
+          → ∀ src tgt : itree modE Any.t,
+            srcs !! cid = Some src → tgts !! cid = Some tgt
+            → ∀ (X : Type) (meta : X) (Q : nat → X → Any.t → Any.t → iProp) (l : list (nat * {X0 : Type & X0})) (itrS itrT : itree hmodE Any.t),
+              (∀ vret ret : Any.t, cid = 0 → Q cid meta vret ret ⊢ ⌜vret = ret⌝) 
+              → paco3 (@elim_rel_def _ ginv stb sk0 _)  bot3 l itrS itrT
+              → src = (if Nat.eq_dec cid cid then Ret () else tau;; Ret ());;; interp_hp itrS
+              → tgt = interp_hp ((if Nat.eq_dec cid cid then Ret () else yield_post ginv sk0);;; vret <- itrT;; inline_hp (prog (SModSem.to_hmod (ginv sk0) (stb sk0) (SMod.modsem md sk0))) (ret <- trigger (Choose Any.t);; trigger (Guarantee (Q cid meta vret ret));;; Ret ret))
+              → base.length srcs = base.length tgts
+              → cid < base.length tgts
+              → (∀ (k : nat) (x y : itree modE Any.t), cid ≠ k → srcs !! k = Some x → tgts !! k = Some y → thread_rel ginv stb md sk0 cid k x y)
+              → r Any.t Any.t eq ps pt
+                  (x <- interp_stateE Any.t (ITree.iter (handle_schE_callE (ModSem.prog (HModSem.to_mod (HModSemAux.inline (SModSemAux.to_hmod (SMod.modsem md sk0))) rs0))) (cid, srcs)) (Any.pair st rs ↑);; Ret x.2)
+                  (x <- interp_stateE Any.t (ITree.iter (handle_schE_callE (ModSem.prog (HModSem.to_mod (HModSemAux.inline (SModSem.to_hmod (ginv sk0) (stb sk0) (SMod.modsem md sk0))) rt0))) (cid, tgts)) (Any.pair st rt ↑);; Ret x.2))
+  :
+  gpaco7 _simg (cpn7 _simg) bot7 r Any.t Any.t eq ps pt
+  (x <- interp_stateE Any.t (tau;; tau;; ITree.iter (handle_schE_callE (ModSem.prog (HModSem.to_mod (HModSemAux.inline (SModSemAux.to_hmod (SMod.modsem md sk0))) rs0)))
+    (cid, <[cid:=interp_hp src]> srcs)) (Any.pair st rs ↑);; Ret x.2)
+  (x <- interp_stateE Any.t (tau;; ITree.iter (handle_schE_callE (ModSem.prog (HModSem.to_mod (HModSemAux.inline (SModSem.to_hmod (ginv sk0) (stb sk0) (SMod.modsem md sk0))) rt0)))
+    (cid, <[cid:=tau;; interp_hp (tau;; x_ <- trigger (Choose X0);; x_0 <-
+                                     (tau;; arg <- trigger (Choose Any.t);;
+                                            (tau;; trigger (Guarantee (P cid x_ varg arg));;;
+                                                   (tau;; tau;; my_tid' <- trigger Tid;;
+                                                                (tau;; x' <- trigger (Take X0);;
+                                                                       (tau;; varg' <- trigger (Take Any.t);;
+                                                                              (tau;; trigger (Assume (P my_tid' x' varg' arg));;; (tau;; Ret (cid, x_, my_tid', x', varg'))))))));;
+                  x_1 <- ktrT x_0;; inline_hp (prog (SModSem.to_hmod (ginv sk0) (stb sk0) (SMod.modsem md sk0))) (ret <- trigger (Choose Any.t);; trigger (Guarantee (Q cid meta x_1 ret));;; Ret ret))]> tgts)) (Any.pair st rt ↑);; Ret x.2).
+  Proof.
+    hide_r. tau 2.
+    reveal ITREE. hide_l. tau 1.
+    iterT 2. iterL. _coreA. ls.
+    iterT 2. iterL. _coreA. ls.
+    iterT 2. iterL. _supd. 
+    iterL. _coreA. iterL. _coreA. ls.
+    iterL. _supd. iterL. _supd.
+    iterT 3. iterL. ls. tau 1.
+    iterT 2. iterL. _coreE x. ls.
+    iterT 2. iterL. _coreE varg. ls.
+    iterT 2.
+    hexploit (Own_bupd_split rt); eauto.
+    i. des.
+    iterL. _coreE a1. ls.
+    iterL. _supd.
+    assert (UPD': Own rs ==∗ Own (a1 ⋅ x1)).
+    {  
+      iIntros "H". iPoseProof (UPD with "H") as ">H".
+      iPoseProof (H with "H") as ">[H0 H1]".
+      iPoseProof (H1 with "H1") as "H1".
+      iModIntro. rewrite Own_op. iFrame.
+    }
+    assert (✓ (a1 ⋅ x1)). 
+    { eapply Own_wand_valid with (a1 := rs); eauto. } 
+    iterL. _coreE H2. ls.
+    iterL. _coreE H0. ls.
+    iterL. _supd. iterL. _supd.
+    iterT 2. 
+    reveal ITREE. prb. gbase. pclearbot.
+    eapply CIH with (l:= _ :: l); eauto; try (rewrite !length_insert; nia); 
+    try (eapply KTR); try (rewrite list_lookup_insert; grind).
+    i. rewrite !list_lookup_insert_ne in H4, H5; eauto.
+  Qed.
+
+  Lemma cancel_main_tail
+    sk0 (SKINCL: incl sk sk0) (SKWF: Sk.wf sk0)
+    X X0 (meta: X) (m: X0) (rs0 rt0 rs rt: Σ) Q Q0 (cid tid: nat) st ps pt l vret
+    src srcs tgts ktrS ktrT
+    (SRC: src = ktrS vret)
+    (LENS: cid < base.length srcs)
+    (LENT: cid < base.length tgts)
+    (LEN: base.length srcs = base.length tgts)
+    (WFS: ✓ rs)
+    (WFT: ✓ rt)
+    (UPD: Own rs ==∗ Own rt)
+    (RET: ∀ vret ret : Any.t, cid = 0 → Q cid meta vret ret ⊢ ⌜vret = ret⌝)
+    (KTR: ∀ vret : Any.t, upaco3 (@elim_rel_def _ ginv stb sk0 _) bot3 l (ktrS vret) (ktrT vret))
+    (RELS: ∀ (k : nat) (x y : itree modE Any.t), cid ≠ k → srcs !! k = Some x → tgts !! k = Some y → thread_rel ginv stb md sk0 cid k x y)
+    (r: ∀ x x0 : Type, (x → x0 → Prop) → smj → smj → itree coreE x → itree coreE x0 → Prop)
+    (CIH: ∀ (rs rt : Σ) (srcs tgts : list (itree modE Any.t)) (cid : nat) (st : Any.t) (ps pt : smj),
+          ✓ rs → cid < base.length srcs → (Own rs ==∗ Own rt) 
+          → ∀ src tgt : itree modE Any.t,
+            srcs !! cid = Some src → tgts !! cid = Some tgt
+            → ∀ (X : Type) (meta : X) (Q : nat → X → Any.t → Any.t → iProp) (l : list (nat * {X0 : Type & X0})) (itrS itrT : itree hmodE Any.t),
+              (∀ vret ret : Any.t, cid = 0 → Q cid meta vret ret ⊢ ⌜vret = ret⌝) 
+              → paco3 (@elim_rel_def _ ginv stb sk0 _)  bot3 l itrS itrT
+              → src = (if Nat.eq_dec cid cid then Ret () else tau;; Ret ());;; interp_hp itrS
+              → tgt = interp_hp ((if Nat.eq_dec cid cid then Ret () else yield_post ginv sk0);;; vret <- itrT;; inline_hp (prog (SModSem.to_hmod (ginv sk0) (stb sk0) (SMod.modsem md sk0))) (ret <- trigger (Choose Any.t);; trigger (Guarantee (Q cid meta vret ret));;; Ret ret))
+              → base.length srcs = base.length tgts
+              → cid < base.length tgts
+              → (∀ (k : nat) (x y : itree modE Any.t), cid ≠ k → srcs !! k = Some x → tgts !! k = Some y → thread_rel ginv stb md sk0 cid k x y)
+              → r Any.t Any.t eq ps pt
+                  (x <- interp_stateE Any.t (ITree.iter (handle_schE_callE (ModSem.prog (HModSem.to_mod (HModSemAux.inline (SModSemAux.to_hmod (SMod.modsem md sk0))) rs0))) (cid, srcs)) (Any.pair st rs ↑);; Ret x.2)
+                  (x <- interp_stateE Any.t (ITree.iter (handle_schE_callE (ModSem.prog (HModSem.to_mod (HModSemAux.inline (SModSem.to_hmod (ginv sk0) (stb sk0) (SMod.modsem md sk0))) rt0))) (cid, tgts)) (Any.pair st rt ↑);; Ret x.2))
+  : 
+  gpaco7 _simg (cpn7 _simg) bot7 r Any.t Any.t eq ps pt
+  (x <- interp_stateE Any.t (tau;; tau;; ITree.iter (handle_schE_callE (ModSem.prog (HModSem.to_mod (HModSemAux.inline (SModSemAux.to_hmod (SMod.modsem md sk0))) rs0)))
+    (cid, <[cid:=interp_hp (tau;; tau;; src)]> srcs)) (Any.pair st rs ↑);; Ret x.2)
+  (x <- interp_stateE Any.t (x_ <- trigger (Choose Any.t);;
+    x_0 <- Ret (inl
+      (cid, <[cid:=lr <- ITree.subst (λ x : Any.t, Ret (inl
+              (vret0 <- ITree.subst (λ x0 : Any.t, tau;; ktrT x0) 
+                        (ITree.subst (λ ret : Any.t, tau;; trigger (Guarantee (Q0 tid m vret ret));;;
+                          (tau;; tau;; tau;; vret0 <- trigger (Take Any.t);; (tau;; trigger (Assume (Q0 tid m vret0 ret));;; (tau;; Ret vret0)))) (Ret x));;
+                          inline_hp (prog (SModSem.to_hmod (ginv sk0) (stb sk0) (SMod.modsem md sk0)))
+                          (ret <- trigger (Choose Any.t);; trigger (Guarantee (Q cid meta vret0 ret));;; Ret ret)))) (Ret x_);;
+                   match lr with
+                   | inl l0 => tau;; interp_hp l0
+                   | inr r0 => Ret r0
+                   end]> tgts));;
+      match x_0 with
+      | inl l0 => tau;; ITree.iter (handle_schE_callE (ModSem.prog (HModSem.to_mod (HModSemAux.inline (SModSem.to_hmod (ginv sk0) (stb sk0) (SMod.modsem md sk0))) rt0))) l0
+      | inr r0 => Ret r0
+      end) (Any.pair st rt ↑);; Ret x.2).
+  Proof.
+    hide_r. tau 2. iterT 2. 
+    reveal ITREE. hide_l. _coreA.
+    iterT 2. iterL. _supd.
+    iterL. _coreA. ls.
+    iterL. _coreA. ls.
+    iterL. _supd. iterL. _supd.
+    iterT 4.
+    iterL. _coreE vret.
+    iterT 2.
+    hexploit (Own_bupd_split rt); eauto.
+    i. des.
+    iterL. _coreE a1. ls.
+    iterL. _supd.
+    assert (UPD': Own rs ==∗ Own (a1 ⋅ x0)). 
+    {  
+      iIntros "H". iPoseProof (UPD with "H") as ">H".
+      iPoseProof (H with "H") as ">[H0 H1]".
+      iPoseProof (H1 with "H1") as "H1".
+      iModIntro. rewrite Own_op. iFrame.
+    }
+    assert (✓ (a1 ⋅ x0)). 
+    { eapply Own_wand_valid with (a1 := rs); eauto. }
+    iterL. _coreE H2. ls.
+    iterL. _coreE H0. ls.
+    iterL. _supd. iterL. _supd.
+    iterT 3. 
+    reveal ITREE. prb. gbase. pclearbot. 
+    eapply CIH; eauto; try (rewrite !length_insert; nia); try (rewrite list_lookup_insert; grind).
+    i. rewrite !list_lookup_insert_ne in H4, H5; eauto.
+  Qed.
+
+
+End CANCEL.
