cancellation/CancelAux3.v
@@ -1,0 +1,204 @@
+Require Import Coqlib.
+Require Import Behavior.
+Require Import AList.
+Require Import SMod2HMod SMod2HModAux.
+Require Import Skeleton.
+Require Import PCM IPM.
+Require Import Any.
+Require Export STB.
+Require Import ModSim ISim HPSim.
+Require Import CtxRefine CtxRefineFacts MainAdequacy ClosedAdequacy.
+Require Import SimGlobal SimGlobalFacts.
+Require Import SMod HMod Mod Events.
+Require Import HModInline ElimRel.
+Require Import Mod2ITree StRed CancelDef.
+
+(* Yield *)
+
+Section CANCEL.
+  Context `{Σ: GRA.t}.
+  Variable ginv: Sk.t -> invspec.
+  Variable stb: Sk.t -> gname -> option fspec.
+  Variable md: SMod.t.
+  Notation iProp := (iProp Σ).
+
+  Let sk: Sk.t := SMod.sk md.
+  Let ms (sk0: Sk.t) (SKINCL: incl sk sk0) (SKWF: Sk.wf sk0) := 
+    SMod.modsem md sk0.
+  Let sbtb (sk0: Sk.t) (SKINCL: incl sk sk0) (SKWF: Sk.wf sk0): alist gname (list string * fspecbody) := 
+    (ms sk0 SKINCL SKWF).(SModSem.fnsems).
+  Let _stb (sk0: Sk.t) (SKINCL: incl sk sk0) (SKWF: Sk.wf sk0): alist gname (list string * fspec) := 
+    List.map (map_snd (fun '(fn, fs) => (fn, fs.(fsb_fspec)))) (sbtb sk0 SKINCL SKWF).
+
+  Hypothesis STBCOMPLETE:
+    forall 
+      sk0 (SKINCL: incl sk sk0) (SKWF: Sk.wf sk0)
+      fn scfsp (FIND: alist_find fn (_stb sk0 SKINCL SKWF) = Some scfsp), stb sk0 fn = Some scfsp.2.
+  Hypothesis STBSOUND:
+    forall 
+      sk0 (SKINCL: incl sk sk0) (SKWF: Sk.wf sk0)
+      fn (FIND: alist_find fn (_stb sk0 SKINCL SKWF) = None),
+      (<<NONE: stb sk0 fn = None>>).
+
+  Let md_src: HMod.t := SModAux.to_hmod md.
+  Let md_tgt: HMod.t := SMod.to_hmod ginv stb md.
+
+  Import CancelTAC.
+
+
+
+  Lemma cancel_main_yield
+    sk0 (SKINCL: incl sk sk0) (SKWF: Sk.wf sk0)
+    X (meta: X) (rs0 rt0 rs rt: Σ) Q (cid tid: nat) st ps pt l
+    srcs tgts ktrS ktrT
+    (LENS: cid < base.length srcs)
+    (LENT: cid < base.length tgts)
+    (LEN: base.length srcs = base.length tgts)
+    (WFS: ✓ rs)
+    (WFT: ✓ rt)
+    (UPD: Own rs ==∗ Own rt)
+    (RET: ∀ vret ret : Any.t, cid = 0 → Q cid meta vret ret ⊢ ⌜vret = ret⌝)
+    (KTR: ∀ (x: ()), upaco3 (@elim_rel_def _ ginv stb sk0 _) bot3 l (ktrS x) (ktrT x))
+    (RELS: ∀ (k : nat) (x y : itree modE Any.t), cid ≠ k → srcs !! k = Some x → tgts !! k = Some y → thread_rel ginv stb md sk0 cid k x y)
+    (r: ∀ x x0 : Type, (x → x0 → Prop) → smj → smj → itree coreE x → itree coreE x0 → Prop)
+    (CIH: ∀ (rs rt : Σ) (srcs tgts : list (itree modE Any.t)) (cid : nat) (st : Any.t) (ps pt : smj),
+          ✓ rs → cid < base.length srcs → (Own rs ==∗ Own rt) 
+          → ∀ src tgt : itree modE Any.t,
+            srcs !! cid = Some src → tgts !! cid = Some tgt
+            → ∀ (X : Type) (meta : X) (Q : nat → X → Any.t → Any.t → iProp) (l : list (nat * {X0 : Type & X0})) (itrS itrT : itree hmodE Any.t),
+              (∀ vret ret : Any.t, cid = 0 → Q cid meta vret ret ⊢ ⌜vret = ret⌝) 
+              → paco3 (@elim_rel_def _ ginv stb sk0 _)  bot3 l itrS itrT
+              → src = (if Nat.eq_dec cid cid then Ret () else tau;; Ret ());;; interp_hp itrS
+              → tgt = interp_hp ((if Nat.eq_dec cid cid then Ret () else yield_post ginv sk0);;; vret <- itrT;; inline_hp (prog (SModSem.to_hmod (ginv sk0) (stb sk0) (SMod.modsem md sk0))) (ret <- trigger (Choose Any.t);; trigger (Guarantee (Q cid meta vret ret));;; Ret ret))
+              → base.length srcs = base.length tgts
+              → cid < base.length tgts
+              → (∀ (k : nat) (x y : itree modE Any.t), cid ≠ k → srcs !! k = Some x → tgts !! k = Some y → thread_rel ginv stb md sk0 cid k x y)
+              → r Any.t Any.t eq ps pt
+                  (x <- interp_stateE Any.t (ITree.iter (handle_schE_callE (ModSem.prog (HModSem.to_mod (HModSemAux.inline (SModSemAux.to_hmod (SMod.modsem md sk0))) rs0))) (cid, srcs)) (Any.pair st rs ↑);; Ret x.2)
+                  (x <- interp_stateE Any.t (ITree.iter (handle_schE_callE (ModSem.prog (HModSem.to_mod (HModSemAux.inline (SModSem.to_hmod (ginv sk0) (stb sk0) (SMod.modsem md sk0))) rt0))) (cid, tgts)) (Any.pair st rt ↑);; Ret x.2))
+  : 
+  gpaco7 _simg (cpn7 _simg) bot7 r Any.t Any.t eq ps pt
+  (x <-
+   interp_stateE Any.t
+     (tau;; ITree.iter (handle_schE_callE (ModSem.prog (HModSem.to_mod (HModSemAux.inline (SModSemAux.to_hmod (SMod.modsem md sk0))) rs0)))
+              (tid, <[cid:=tau;; interp_hp (ktrS ())]> srcs)) (Any.pair st rs ↑);; Ret x.2)
+  (x <-
+   interp_stateE Any.t
+     (x_ <- trigger sGet;;
+      x_0 <-
+      Ret
+        (inl
+           (cid,
+            <[cid:=lr <-
+                   ITree.subst
+                     (λ x : (),
+                        Ret
+                          (inl
+                             (vret <-
+                              ITree.subst (λ x0 : (), ktrT x0)
+                                (ITree.subst (λ _ : (), tau;; trigger (Yield tid);;; (tau;; my_tid <- trigger Tid;; (tau;; trigger (Assume (ginv sk0 my_tid))))) (Ret x));;
+                              inline_hp (prog (SModSem.to_hmod (ginv sk0) (stb sk0) (SMod.modsem md sk0)))
+                                (ret <- trigger (Choose Any.t);; trigger (Guarantee (Q cid meta vret ret));;; Ret ret))))
+                     (ITree.subst (λ mr : Σ, mr' <- trigger (Choose Σ);; guarantee (Own mr ==∗ ginv sk0 tid ∗ Own mr');;; mput_res mr')
+                        (ITree.subst (λ st0 : Any.t, x_0 <- (Any.split st0) ?;; (let (_, mr) := x_0 in (mr ↓) ?)) (Ret x_)));;
+                   match lr with
+                   | inl l0 => tau;; interp_hp l0
+                   | inr r0 => Ret r0
+                   end]> tgts));;
+      match x_0 with
+      | inl l0 => tau;; ITree.iter (handle_schE_callE (ModSem.prog (HModSem.to_mod (HModSemAux.inline (SModSem.to_hmod (ginv sk0) (stb sk0) (SMod.modsem md sk0))) rt0))) l0
+      | inr r0 => Ret r0
+      end) (Any.pair st rt ↑);; Ret x.2).
+  Proof.
+    hide_r. tau 1.
+    reveal ITREE. hide_l.
+    _supd. iterL. _coreA. ls. iterL. _coreA. ls.
+    iterL. _supd. iterL. _supd.
+    iterT 2. iterL. tau 1. ls.  
+    hexploit (Own_bupd_split rt); eauto. i. des.
+    assert (UPD': Own rs ==∗ Own (a1 ⋅ x)). 
+    {
+      iIntros "H". iPoseProof (UPD with "H") as ">H".
+      iPoseProof (H with "H") as ">[H0 H1]".
+      iModIntro. iSplitL "H0"; eauto.
+      iApply H1; eauto.
+    }
+    assert (✓ (a1 ⋅ x)). 
+    { eapply Own_wand_valid with (a1 := rs); eauto. } 
+    destruct (Nat.eq_dec cid tid).
+    {
+      (* yield to itself *)
+      subst tid.
+      iterT 2. iterL. tau 1. iterT 2.
+      iterL. _coreE a1. iterL. _supd.
+      iterL. _coreE H2. ls.
+      iterL. _coreE H0. ls.
+      iterL. _supd. iterL. _supd. 
+      iterT 1.
+      reveal ITREE. hide_r. iterT 1. reveal ITREE.
+      prb. gbase. pclearbot. 
+      eapply CIH; try (rewrite !length_insert; eauto); try (rewrite list_lookup_insert; grind); eauto; grind.
+      rewrite !list_lookup_insert_ne in H4, H5; eauto.
+    }
+    destruct (classic (tid < base.length srcs)); cycle 1.
+    {
+      reveal ITREE. 
+      hide_r. eapply Nat.le_ngt, lookup_ge_None_2 in H3.
+      _iter. rewrite list_lookup_insert_ne; [|et]. rewrite H3.
+      s. unfold triggerUB. ired. _coreA.
+    } 
+    exploit lookup_lt_is_Some_2; eauto. i. inv x2.
+    exploit (lookup_lt_is_Some_2 tgts tid); [nia|]. i. inv x3.
+    assert (tid < base.length tgts) by nia.
+    hexploit RELS; eauto. i. 
+    depdes H7.
+    (* move to another thread *)
+    destruct (Nat.eq_dec tid cid); try nia.
+    subst. _iter.  
+    replace (<[cid:=tau;; interp_hp
+    (tau;; ' r0 : nat <- trigger Tid;;
+           ' x1 : () <- (tau;; trigger (Assume (ginv sk0 r0)));;
+           ' x2 : Any.t <- ktrT x1;;
+           inline_hp (prog (SModSem.to_hmod (ginv sk0) (stb sk0) (SMod.modsem md sk0)))
+             (' ret : Any.t <- trigger (Choose Any.t);; trigger (Guarantee (Q  cid meta x2 ret));;; Ret ret))]> tgts !! tid)
+    with (tgts !! tid) by (rewrite list_lookup_insert_ne; eauto).
+    rewrite H5. ired. tau 2.
+    iterT 1. iterL. tau 1. ls. iterT 2. 
+    iterL. _coreE a1. ls. iterL. _supd.
+    iterL. _coreE H2. ls. iterL. _coreE H0. ls.
+    iterL. _supd. iterL. _supd. 
+    reveal ITREE. prb. gbase. pclearbot. 
+    eapply CIH with (Q:=Q0); try (rewrite !length_insert; eauto); try (rewrite list_lookup_insert; grind); swap 1 6.
+    { 
+      instantiate (1:= tau;; itrT). instantiate (1:= tau;; itrS).
+      pstep. econs. eauto.
+    }
+    all: eauto.
+    {
+      des_ifs. grind. rewrite list_lookup_insert_ne; eauto.
+      rewrite H4 interp_hp_tau. grind. 
+    }
+    { rewrite length_insert. nia. }
+    { des_ifs. rewrite -interp_hp_tau. grind. }
+    i. destruct (Nat.eq_dec cid k); cycle 1.
+    {
+      rewrite !list_lookup_insert_ne in H8, H9; eauto.
+      hexploit RELS; eauto. i. depdes H10; econs; eauto.
+      { rewrite SRC. des_ifs. }
+      rewrite TGT. des_ifs.
+    }
+    subst k.
+    rewrite list_lookup_insert_ne in H9; eauto.
+    rewrite list_lookup_insert in H8; eauto.
+    rewrite list_lookup_insert in H9; eauto.
+    inv H8. econs; try refl; grind; eauto.
+    rewrite/yield_post -interp_hp_tau.
+    f_equal. ired. do 5 f_equal. 
+    extensionalities. ired. do 3 f_equal.
+    extensionalities. ired. f_equal.
+    destruct H9. eauto.
+  Qed.
+
+  
+
+End CANCEL.
